Strata/DL/Imperative.lean
@@ -12,7 +12,10 @@ public import Strata.DL.Imperative.MetaData
 public import Strata.DL.Imperative.CmdEval
 public import Strata.DL.Imperative.CmdType
 public import Strata.DL.Imperative.CmdSemantics
+public import Strata.DL.Imperative.CmdSemanticsProps
+public import Strata.DL.Imperative.StmtProps
 public import Strata.DL.Imperative.StmtSemantics
+public import Strata.DL.Imperative.StmtSemanticsProps
 
 public import Strata.DL.Imperative.KleeneStmt
 public import Strata.DL.Imperative.KleeneStmtSemantics
