Strata/Languages/C_Simp/Verify.lean
@@ -38,6 +38,13 @@ def translate_opt_expr (e : Option C_Simp.Expression.Expr) : Option (Lambda.LExp
   | some e => translate_expr e
   | none => none
 
+def translate_opt_labeled_expr
+    (e : Option (String × C_Simp.Expression.Expr)) :
+    Option (String × Lambda.LExpr Core.CoreLParams.mono) :=
+  match e with
+  | some (l, e) => some (l, translate_expr e)
+  | none => none
+
 def translate_cmd (c: C_Simp.Command) : Core.Command :=
   match c with
   | .init name ty e _md =>
@@ -57,7 +64,7 @@ def translate_stmt (s: Imperative.Stmt C_Simp.Expression C_Simp.Command) : Core.
   | .ite cond thenb elseb _md =>
     .ite (cond.map translate_expr) (thenb.map translate_stmt) (elseb.map translate_stmt) {}
   | .loop guard measure invariant body _md =>
-    .loop (guard.map translate_expr) (translate_opt_expr measure)
+    .loop (guard.map translate_expr) (translate_opt_labeled_expr measure)
       (invariant.map (fun (l, e) => (l, translate_expr e))) (body.map translate_stmt) {}
   | .funcDecl _ _ => panic! "C_Simp does not support function declarations"
   | .typeDecl _ _ => panic! "C_Simp does not support type declarations"
@@ -87,7 +94,7 @@ def loop_elimination_statement(s : C_Simp.Statement) : Core.Statement :=
   match s with
   | .loop guard measure invList body _ =>
     match guard, measure, invList with
-    | .det guard_expr, .some measure, _ =>
+    | .det guard_expr, .some (_, measure), _ =>
       let assigned_vars := (Imperative.Block.modifiedVars body).map (λ s => ⟨s.name, ()⟩)
       let havocd : Core.Statement := .block "loop havoc" (assigned_vars.map (λ n => Core.Statement.havoc n {})) {}
 
